experiment/Experiment.Steel.Repr.ST.fst
@@ -4,46 +4,33 @@ module U    = Learn.Util
 module M    = Experiment.Steel.Repr.M
 module L    = FStar.List.Pure
 module Uv   = FStar.Universe
+module Dl   = Learn.DList
 module Perm = Learn.Permutation
 
 open Experiment.Steel.Repr.M
 open Steel.Effect.Common
 
 
-(* TODO? define vequiv for [list a] *)
-let vequiv (ts0 ts1 : ty_list) = f : Perm.perm_f (L.length ts0) {ts1 == Perm.apply_perm_r f ts0}
-
-unfold
-let apply_vequiv (#ts0 #ts1 : ty_list) (f : vequiv ts0 ts1) (xs : var_list ts0) : var_list ts1
-  = var_apply_perm_r f xs
-
-unfold
-let var_split_at_ty (ts0 ts1 : ty_list) (xs : var_list L.(ts0@ts1))
-  : var_list ts0 & var_list ts1
-  = L.lemma_append_splitAt ts0 ts1;
-    var_splitAt (L.length ts0) xs
-
-
-type pre_t = ty_list
-type post_t (a : Type) = a -> ty_list
-type req_t (pre : pre_t) = var_list pre -> prop
-type ens_t (pre : pre_t) (a : Type) (post : post_t a) = var_list pre -> (x : a) -> var_list (post x) -> prop
+type pre_t = Dl.ty_list
+type post_t (a : Type) = a -> Dl.ty_list
+type req_t (pre : pre_t) = Dl.dlist pre -> prop
+type ens_t (pre : pre_t) (a : Type) (post : post_t a) = Dl.dlist pre -> (x : a) -> Dl.dlist (post x) -> prop
 
 
 type unit' : Type u#a = | Unit' : unit'
 
 noeq
 type prog_tree : (a : Type u#a) -> (pre : pre_t u#b) -> (post : post_t u#a u#b a) -> Type u#(1 + max a b) =
-  | Tequiv : (pre : ty_list) -> (post : ty_list) ->
-             (p : vequiv pre post) ->
+  | Tequiv : (pre : Dl.ty_list) -> (post : Dl.ty_list) ->
+             (p : Perm.pequiv pre post) ->
              prog_tree unit' pre (fun _ -> post)
-  | Tspec  : (a : Type u#a) -> (pre : pre_t) -> (post : post_t a) -> (frame : ty_list) ->
+  | Tspec  : (a : Type u#a) -> (pre : pre_t) -> (post : post_t a) -> (frame : Dl.ty_list) ->
              (req : req_t pre) -> (ens : ens_t pre a post) ->
              prog_tree a L.(pre@frame) (fun (x : a) -> L.(post x @ frame))
   | Tret   : (a : Type u#a) -> (x : a) -> (post : post_t a) ->
              prog_tree a (post x) post
   | Tbind  : (a : Type u#a) -> (b : Type u#a) ->
-             (pre : pre_t) -> (itm : (a -> ty_list)) -> (post : post_t b) ->
+             (pre : pre_t) -> (itm : (a -> Dl.ty_list)) -> (post : post_t b) ->
              (f : prog_tree a pre itm) -> (g : ((x : a) -> prog_tree b (itm x) post)) ->
              prog_tree b pre post
   | TbindP : (a : Type u#a) -> (b : Type u#a) ->
@@ -51,7 +38,7 @@ type prog_tree : (a : Type u#a) -> (pre : pre_t u#b) -> (post : post_t u#a u#b a
              (wp : pure_wp a) -> (x : unit -> PURE a wp) -> (g : a -> prog_tree b pre post) ->
              prog_tree b pre post
 
-let bind (#a : Type) (#b : Type) (#pre : pre_t) (#itm : a -> ty_list) (#post : post_t b)
+let bind (#a : Type) (#b : Type) (#pre : pre_t) (#itm : a -> Dl.ty_list) (#post : post_t b)
          (f : prog_tree a pre itm) (g : (x:a) -> prog_tree b (itm x) post)
   : prog_tree b pre post
   = Tbind a b pre itm post f g
@@ -63,12 +50,12 @@ let rec tree_req (#a : Type) (#pre : pre_t) (#post : post_t a) (t : prog_tree a 
   | Tequiv _ _ _ ->
              (fun sl0 -> True)
   | Tspec _  pre _ frame  req _ ->
-             (fun sl0 -> req (var_split_at_ty pre frame sl0)._1)
+             (fun sl0 -> req (Dl.splitAt_ty pre frame sl0)._1)
   | Tret _ _ _ ->
              (fun sl0 -> True)
   | Tbind a _  _ itm _  f g ->
              (fun sl0 -> tree_req f sl0 /\
-               (forall (x : a) (sl1 : var_list (itm x)) . tree_ens f sl0 x sl1 ==> tree_req (g x) sl1))
+               (forall (x : a) (sl1 : Dl.dlist (itm x)) . tree_ens f sl0 x sl1 ==> tree_req (g x) sl1))
   | TbindP a _  _ _  wp _ g ->
              (fun sl0 -> wp (fun (x : a) -> tree_req (g x) sl0) /\ True)
 
@@ -76,17 +63,17 @@ and tree_ens (#a : Type) (#pre : pre_t) (#post : post_t a) (t : prog_tree a pre 
   : Tot (ens_t pre a post) (decreases t)
   = match t with
   | Tequiv _ _ p ->
-             (fun sl0 _ sl1 -> sl1 == apply_vequiv p sl0)
+             (fun sl0 _ sl1 -> sl1 == Dl.apply_pequiv p sl0)
   | Tspec _  pre post frame  req ens ->
              (fun sl0 x sl1 ->
-               let sl0', frame0 = var_split_at_ty pre      frame sl0 in
-               let sl1', frame1 = var_split_at_ty (post x) frame sl1 in
+               let sl0', frame0 = Dl.splitAt_ty pre      frame sl0 in
+               let sl1', frame1 = Dl.splitAt_ty (post x) frame sl1 in
                frame1 == frame0 /\ ens sl0' x sl1')
   | Tret _ x post ->
              (fun sl0 x' sl1 -> x' == x /\ sl1 == sl0)
   | Tbind a _  _ itm _  f g ->
              (fun sl0 y sl2 -> tree_req f sl0 /\
-               (exists (x : a) (sl1 : var_list (itm x)) . tree_ens f sl0 x sl1 /\ tree_ens (g x) sl1 y sl2))
+               (exists (x : a) (sl1 : Dl.dlist (itm x)) . tree_ens f sl0 x sl1 /\ tree_ens (g x) sl1 y sl2))
   | TbindP a _  _ _  wp _ g ->
              (fun sl0 y sl1 -> as_requires wp /\ (exists (x : a) . as_ensures wp x /\ tree_ens (g x) sl0 y sl1))
 
@@ -96,29 +83,21 @@ and tree_ens (#a : Type) (#pre : pre_t) (#post : post_t a) (t : prog_tree a pre 
 module T = FStar.Tactics
 open FStar.Calc
 
-unfold
-let vequiv_of_M (#src #dst : vprop_list) (p : M.vequiv src dst)
-  : Pure (vequiv (vprop_list_sels_t src) (vprop_list_sels_t dst))
-         (requires True) (ensures fun p' ->
-           U.cast #(Perm.perm_f (L.length (vprop_list_sels_t src))) (Perm.perm_f (L.length src)) p' == p)
-  = Perm.map_apply_r p Mkvprop'?.t src;
-    U.cast #(Perm.perm_f (L.length src)) (Perm.perm_f (L.length (vprop_list_sels_t src))) p
-
 let rec repr_ST_of_M (#a : Type u#a) (t : M.prog_tree a)
                      (#pre : M.pre_t) (#post : M.post_t a) (c : M.tree_cond t pre post)
   : Tot (prog_tree a (vprop_list_sels_t pre) (fun (x : a) -> vprop_list_sels_t (post x)))
         (decreases t)
   = match c with
   | TCspec #a #pre #post #req #ens  pre' post' frame  p0 p1 ->
-             Tequiv (vprop_list_sels_t pre') (vprop_list_sels_t L.(pre@frame)) (vequiv_of_M p0);;
+             Tequiv (vprop_list_sels_t pre') (vprop_list_sels_t L.(pre@frame)) (vequiv_sl p0);;
              (**) L.map_append Mkvprop'?.t pre frame;
              x <-- Tspec a (vprop_list_sels_t pre) (fun (x : a) -> vprop_list_sels_t (post x))
                           (vprop_list_sels_t frame) req ens;
              (**) L.map_append Mkvprop'?.t (post x) frame;
-             Tequiv (vprop_list_sels_t L.(post x@frame)) (vprop_list_sels_t (post' x)) (vequiv_of_M (p1 x));;
+             Tequiv (vprop_list_sels_t L.(post x@frame)) (vprop_list_sels_t (post' x)) (vequiv_sl (p1 x));;
              Tret _ x (fun x -> vprop_list_sels_t (post' x))
   | TCret #a #x  pre post  p ->
-             Tequiv (vprop_list_sels_t pre) (vprop_list_sels_t (post x)) (vequiv_of_M p);;
+             Tequiv (vprop_list_sels_t pre) (vprop_list_sels_t (post x)) (vequiv_sl p);;
              Tret _ x (fun x -> vprop_list_sels_t (post x))
   | TCbind #a #b #f #g  pre itm post  cf cg ->
              x <-- repr_ST_of_M f cf;
@@ -131,45 +110,11 @@ let norm_tree_spec () : T.Tac unit
   = T.norm [delta_only [`%repr_ST_of_M; `%bind; `%tree_req; `%tree_ens];
             zeta; iota; simplify]
 
-unfold
-let vequiv_sym (#ts0 #ts1 : ty_list) (f : vequiv ts0 ts1) : vequiv ts1 ts0
-  = 
-    Perm.(calc (==) {
-      apply_perm_r (inv_f f) ts1;
-    == {}
-      apply_perm_r (inv_f f) (apply_perm_r f ts0);
-    == {apply_r_comp (inv_f f) f ts0}
-      ts0;
-    });
-    U.cast #(Perm.perm_f (L.length ts0)) (Perm.perm_f (L.length ts1)) (Perm.inv_f f)
-
-let vequiv_ts_eq (#ts0 #ts1 : ty_list) (f : vequiv ts0 ts1)
-  : Lemma (ts1 == Perm.apply_perm_r f ts0)
-  = ()
-
-let apply_vequiv_sym_l (#ts0 #ts1 : ty_list) (f : vequiv ts0 ts1) (xs : var_list ts0)
-  : Lemma (apply_vequiv (vequiv_sym f) (apply_vequiv f xs) == xs)
-  =
-    var_apply_r_comp (Perm.inv_f f) f xs
-
-let apply_vequiv_sym_r (#ts0 #ts1 : ty_list) (f : vequiv ts0 ts1) (xs : var_list ts1)
-  : Lemma (apply_vequiv f (apply_vequiv (vequiv_sym f) xs) == xs)
-  =
-    vequiv_ts_eq (vequiv_sym f);
-    var_apply_r_comp f (Perm.inv_f f) xs
-
-
-let apply_vequiv_sym_eq_iff (#ts0 #ts1 : ty_list) (f : vequiv ts0 ts1) (xs : var_list ts0) (ys : var_list ts1)
-  : Lemma (xs == apply_vequiv (vequiv_sym f) ys <==> ys == apply_vequiv f xs)
-  =
-    apply_vequiv_sym_l f xs;
-    apply_vequiv_sym_r f ys
-
 #push-options "--z3rlimit 15"
 let repr_ST_of_M__TCspec_ens
       #a #pre #post (req : M.req_t pre) (ens : M.ens_t pre a post)
       (pre' : M.pre_t) (post' : M.post_t a) (frame : vprop_list)
-      (p0 : M.vequiv pre' L.(pre @ frame)) (p1 : (x : a) -> M.vequiv (post x @ frame) (post' x))
+      (p0 : vequiv pre' L.(pre @ frame)) (p1 : (x : a) -> vequiv (post x @ frame) (post' x))
       (sl0' : sl_t pre') (res : a) (sl1' : sl_t (post' res))
 
   : Lemma (
@@ -177,34 +122,34 @@ let repr_ST_of_M__TCspec_ens
     (**) L.map_append Mkvprop'?.t (post res) frame;
 
     (tree_ens (repr_ST_of_M _ (TCspec #a #pre #post #req #ens  pre' post' frame  p0 p1)) sl0' res sl1'
-    <==> (let sl0, frame0 = var_split_at_ty (vprop_list_sels_t pre) (vprop_list_sels_t frame)
-                             (apply_vequiv (vequiv_of_M p0) sl0') in
-        let sl1, frame1 = var_split_at_ty (vprop_list_sels_t (post res)) (vprop_list_sels_t frame)
-                             (apply_vequiv (vequiv_sym (vequiv_of_M (p1 res))) sl1') in
+    <==> (let sl0, frame0 = Dl.splitAt_ty (vprop_list_sels_t pre) (vprop_list_sels_t frame)
+                             (Dl.apply_pequiv (vequiv_sl p0) sl0') in
+        let sl1, frame1 = Dl.splitAt_ty (vprop_list_sels_t (post res)) (vprop_list_sels_t frame)
+                             (Dl.apply_pequiv (Perm.pequiv_sym (vequiv_sl (p1 res))) sl1') in
         req sl0 /\ frame1 == frame0 /\ ens sl0 res sl1)))
   =
     L.map_append Mkvprop'?.t pre frame;
     L.map_append Mkvprop'?.t (post res) frame;
     assert (
       tree_ens (repr_ST_of_M _ (TCspec #a #pre #post #req #ens  pre' post' frame  p0 p1)) sl0' res sl1'
-    <==> (exists (sl1f : var_list L.(vprop_list_sels_t (post res) @ vprop_list_sels_t frame)) .
-          let sl0, frame0 = var_split_at_ty (vprop_list_sels_t pre) (vprop_list_sels_t frame)
-                               (apply_vequiv (vequiv_of_M p0) sl0') in
-          let sl1, frame1 = var_split_at_ty (vprop_list_sels_t (post res)) (vprop_list_sels_t frame) sl1f in
-          sl1' == apply_vequiv (vequiv_of_M (p1 res)) sl1f /\
+    <==> (exists (sl1f : Dl.dlist L.(vprop_list_sels_t (post res) @ vprop_list_sels_t frame)) .
+          let sl0, frame0 = Dl.splitAt_ty (vprop_list_sels_t pre) (vprop_list_sels_t frame)
+                               (Dl.apply_pequiv (vequiv_sl p0) sl0') in
+          let sl1, frame1 = Dl.splitAt_ty (vprop_list_sels_t (post res)) (vprop_list_sels_t frame) sl1f in
+          sl1' == Dl.apply_pequiv (vequiv_sl (p1 res)) sl1f /\
           req sl0 /\ frame1 == frame0 /\ ens sl0 res sl1))
       by T.(norm_tree_spec (); smt ());
     
-    introduce forall (sl1f : var_list L.(vprop_list_sels_t (post res) @ vprop_list_sels_t frame)) .
-        sl1' == apply_vequiv (vequiv_of_M (p1 res)) sl1f <==>
-        sl1f == apply_vequiv (vequiv_sym (vequiv_of_M (p1 res))) sl1'
-      with apply_vequiv_sym_eq_iff (vequiv_of_M (p1 res)) sl1f sl1';
+    introduce forall (sl1f : Dl.dlist L.(vprop_list_sels_t (post res) @ vprop_list_sels_t frame)) .
+        sl1' == Dl.apply_pequiv (vequiv_sl (p1 res)) sl1f <==>
+        sl1f == Dl.apply_pequiv (Perm.pequiv_sym (vequiv_sl (p1 res))) sl1'
+      with Dl.apply_pequiv_sym_eq_iff (vequiv_sl (p1 res)) sl1f sl1';
 
     assert (tree_ens (repr_ST_of_M _ (TCspec #a #pre #post #req #ens  pre' post' frame  p0 p1)) sl0' res sl1'
-    <==> (let sl0, frame0 = var_split_at_ty (vprop_list_sels_t pre) (vprop_list_sels_t frame)
-                             (apply_vequiv (vequiv_of_M p0) sl0') in
-        let sl1, frame1 = var_split_at_ty (vprop_list_sels_t (post res)) (vprop_list_sels_t frame)
-                             (apply_vequiv (vequiv_sym (vequiv_of_M (p1 res))) sl1') in
+    <==> (let sl0, frame0 = Dl.splitAt_ty (vprop_list_sels_t pre) (vprop_list_sels_t frame)
+                             (Dl.apply_pequiv (vequiv_sl p0) sl0') in
+        let sl1, frame1 = Dl.splitAt_ty (vprop_list_sels_t (post res)) (vprop_list_sels_t frame)
+                             (Dl.apply_pequiv (Perm.pequiv_sym (vequiv_sl (p1 res))) sl1') in
         req sl0 /\ frame1 == frame0 /\ ens sl0 res sl1))
 #pop-options
 
@@ -225,13 +170,13 @@ let rec repr_ST_of_M_req (#a : Type) (t : M.prog_tree a)
              <==> {_ by T.(apply_lemma (`U.iff_refl); trefl ()) }
                req (extract_vars_f pre' pre frame p0 sl0)._1;
              <==> { assert_norm (extract_vars_f pre' pre frame p0 sl0
-                    == var_split_at_ty (vprop_list_sels_t pre) (vprop_list_sels_t frame)
-                         (apply_vequiv (vequiv_of_M p0) sl0)) }
-               req (var_split_at_ty (vprop_list_sels_t pre) (vprop_list_sels_t frame)
-                              (apply_vequiv (vequiv_of_M p0) sl0))._1;
+                    == Dl.splitAt_ty (vprop_list_sels_t pre) (vprop_list_sels_t frame)
+                         (Dl.apply_pequiv (vequiv_sl p0) sl0)) }
+               req (Dl.splitAt_ty (vprop_list_sels_t pre) (vprop_list_sels_t frame)
+                              (Dl.apply_pequiv (vequiv_sl p0) sl0))._1;
              <==> { assert (tree_req (repr_ST_of_M _ (TCspec #a #pre #post #req #ens  pre' post' frame  p0 p1)) sl0
-                     <==> req (var_split_at_ty (vprop_list_sels_t pre) (vprop_list_sels_t frame)
-                              (apply_vequiv (vequiv_of_M p0) sl0))._1)
+                     <==> req (Dl.splitAt_ty (vprop_list_sels_t pre) (vprop_list_sels_t frame)
+                              (Dl.apply_pequiv (vequiv_sl p0) sl0))._1)
                  by T.(norm_tree_spec (); smt ()) }
                tree_req (repr_ST_of_M _ (TCspec #a #pre #post #req #ens  pre' post' frame  p0 p1)) sl0;
              <==> { U.f_equal tree_req (repr_ST_of_M _ (TCspec #a #pre #post #req #ens  pre' post' frame  p0 p1))
@@ -265,7 +210,7 @@ let rec repr_ST_of_M_req (#a : Type) (t : M.prog_tree a)
                with _ . (repr_ST_of_M_ens f cf sl0 x sl1; repr_ST_of_M_req (g x) (cg x) sl1)
              }
                tree_req (repr_ST_of_M f cf) sl0 /\
-               (forall (x : a) (sl1 : var_list (vprop_list_sels_t (itm x))) .
+               (forall (x : a) (sl1 : Dl.dlist (vprop_list_sels_t (itm x))) .
                  tree_ens (repr_ST_of_M f cf) sl0 x sl1 ==> tree_req (repr_ST_of_M (g x) (cg x)) sl1);
              <==> {_ by T.(apply_lemma (`U.iff_refl); trefl ())}
                tree_req (repr_ST_of_M _ (TCbind #a #b #f #g  pre itm post  cf cg)) sl0;
@@ -309,13 +254,13 @@ and repr_ST_of_M_ens (#a : Type) (t : M.prog_tree a)
                M.tree_ens _ (TCspec #a #pre #post #req #ens  pre' post' frame  p0 p1) sl0 res sl1;
              <==> {_ by T.(apply_lemma (`U.iff_refl); trefl ()) }
               (let fsl0, frame0 = extract_vars_f pre' pre frame p0 sl0 in
-               let fsl1, frame1 = extract_vars_f (post' res) (post res) frame (M.vequiv_sym (p1 res)) sl1 in
+               let fsl1, frame1 = extract_vars_f (post' res) (post res) frame (Perm.pequiv_sym (p1 res)) sl1 in
                 frame1 == frame0 /\ ens fsl0 res fsl1);
              <==> { (* since req holds *) }
-              (let fsl0, frame0 = var_split_at_ty (vprop_list_sels_t pre) (vprop_list_sels_t frame)
-                                                  (apply_vequiv (vequiv_of_M p0) sl0) in
-               let fsl1, frame1 = var_split_at_ty (vprop_list_sels_t (post res)) (vprop_list_sels_t frame)
-                                                  (apply_vequiv (vequiv_sym (vequiv_of_M (p1 res))) sl1) in
+              (let fsl0, frame0 = Dl.splitAt_ty (vprop_list_sels_t pre) (vprop_list_sels_t frame)
+                                                  (Dl.apply_pequiv (vequiv_sl p0) sl0) in
+               let fsl1, frame1 = Dl.splitAt_ty (vprop_list_sels_t (post res)) (vprop_list_sels_t frame)
+                                                  (Dl.apply_pequiv (Perm.pequiv_sym (vequiv_sl (p1 res))) sl1) in
                 req fsl0 /\ frame1 == frame0 /\ ens fsl0 res fsl1);
              <==> {repr_ST_of_M__TCspec_ens req ens pre' post' frame p0 p1 sl0 res sl1}
                tree_ens (repr_ST_of_M _ (TCspec #a #pre #post #req #ens  pre' post' frame p0 p1)) sl0 res sl1;
@@ -332,9 +277,9 @@ and repr_ST_of_M_ens (#a : Type) (t : M.prog_tree a)
                       by T.(norm [delta_only [`%M.tree_ens]; zeta; iota]; smt ()) }
                res == x /\ sl1 == extract_vars p sl0;
              <==> {}
-               res == x /\ sl1 == apply_vequiv (vequiv_of_M p) sl0;
+               res == x /\ sl1 == Dl.apply_pequiv (vequiv_sl p) sl0;
              <==> { assert (tree_ens (repr_ST_of_M _ (TCret #a #x pre post p)) sl0 res sl1 <==>
-                           (res == x /\ sl1 == apply_vequiv (vequiv_of_M p) sl0))
+                           (res == x /\ sl1 == Dl.apply_pequiv (vequiv_sl p) sl0))
                       by T.(norm_tree_spec (); smt ()) }
                tree_ens (repr_ST_of_M _ (TCret #a #x pre post p)) sl0 res sl1;
              <==> { U.f_equal tree_ens (repr_ST_of_M _ (TCret #a #x pre post p))
@@ -360,7 +305,7 @@ and repr_ST_of_M_ens (#a : Type) (t : M.prog_tree a)
                 with _ . repr_ST_of_M_ens (g x) (cg x) sl1' res sl1
              }
                tree_req (repr_ST_of_M f cf) sl0 /\
-               (exists (x : a) (sl1' : var_list (vprop_list_sels_t (itm x))) .
+               (exists (x : a) (sl1' : Dl.dlist (vprop_list_sels_t (itm x))) .
                  tree_ens (repr_ST_of_M f cf) sl0 x sl1' /\
                  tree_ens (repr_ST_of_M (g x) (cg x)) sl1' res sl1);
              <==> {_ by T.(apply_lemma (`U.iff_refl); trefl ())}
