pure/Learn.DList.fst
@@ -1,0 +1,158 @@
+module Learn.DList
+
+module U    = Learn.Util
+module L    = FStar.List.Pure
+module Ll   = Learn.List
+module Perm = Learn.Permutation
+
+(*** Dependent lists *)
+
+type ty_list = list Type
+
+noeq
+type dlist : ty_list -> Type =
+  | DNil : dlist []
+  | DCons : (t0 : Type) -> (x0 : t0) ->
+             (ts : ty_list) -> (xs : dlist ts) ->
+             dlist (t0 :: ts)
+
+
+let rec index (#ts : ty_list) (xs : dlist ts) (i : nat{i < L.length ts})
+  : L.index ts i
+  = let DCons t0 x0 ts1 xs1 = xs in
+    if i = 0 then x0
+    else U.cast (L.index ts i) (index xs1 (i-1))
+
+let rec dlist_extensionality (#ts : ty_list) (xs ys : dlist ts)
+  : Lemma (requires forall (i : nat {i < L.length ts}) . index xs i == index ys i)
+          (ensures xs == ys)
+          (decreases ts)
+  = match ts with
+    | [] -> ()
+    | t0 :: ts' -> let DCons _ x _ xs' = xs in
+                let DCons _ y _ ys' = ys in
+                assert (x == index xs 0);
+                assert (y == index ys 0);
+                introduce forall (i : nat {i < L.length ts'}) . index xs' i == index ys' i
+                  with (assert (index xs' i === index xs (i+1));
+                        assert (index ys' i === index ys (i+1)));
+                dlist_extensionality #ts' xs' ys'
+
+
+let rec splitAt (n : nat) (#ts : ty_list) (xs : dlist ts)
+  : Tot (dlist (L.splitAt n ts)._1 & dlist (L.splitAt n ts)._2)
+        (decreases n)
+  = if n = 0 then DNil, xs
+    else match xs with
+    | DNil              -> DNil, DNil
+    | DCons t0 x0 ts xs -> let xs0, xs1 = splitAt (n-1) xs in
+                           DCons t0 x0 _ xs0, xs1
+
+let rec splitAt_ty (ts0 ts1 : ty_list) (xs : dlist L.(ts0@ts1))
+  : Tot (dlist ts0 & dlist ts1) (decreases ts0)
+  = match ts0 with
+    | [] -> DNil, xs
+    | t0 :: ts0 -> let DCons _ x0 _ xs = xs in
+                 let xs0, xs1 = splitAt_ty ts0 ts1 xs in
+                 DCons t0 x0 _ xs0, xs1
+
+let rec splitAt_ty_eq (ts0 ts1 : ty_list) (xs : dlist L.(ts0@ts1))
+  : Lemma (ensures L.(splitAt (length ts0) (ts0@ts1) == (ts0, ts1)) /\
+                   splitAt_ty ts0 ts1 xs == splitAt L.(length ts0) xs)
+          (decreases ts0)
+  = match ts0 with
+  | [] -> ()
+  | t0 :: ts0 -> let DCons _ x0 _ xs = xs in splitAt_ty_eq ts0 ts1 xs
+
+
+let rec initi (lb ub : nat)
+          (t : (i:nat{lb <= i /\ i < ub}) -> Tot Type)
+          (f : (i:nat{lb <= i /\ i < ub}) -> Tot (t i))
+  : Tot (dlist (Ll.initi lb ub t)) (decreases ub - lb)
+  = if lb < ub then DCons (t lb) (f lb) _ (initi (lb + 1) ub t f) else DNil
+
+let rec initi_at (lb ub : nat)
+          (t : (i:nat{lb <= i /\ i < ub}) -> Tot Type)
+          (f : (i:nat{lb <= i /\ i < ub}) -> Tot (t i))
+          (i : nat {i < L.length (Ll.initi lb ub t)})
+  : Lemma (ensures index (initi lb ub t f) i == f (lb+i)) (decreases i)
+          [SMTPat (index (initi lb ub t f) i)]
+  = if i = 0 then () else initi_at (lb+1) ub t f (i-1)
+
+
+(** permutations *)
+
+let apply_perm_r (#n : nat) (p : Perm.perm_f n) (#ts : ty_list {L.length ts == n}) (xs : dlist ts)
+  : dlist (Perm.apply_perm_r p ts)
+  = initi 0 n (fun i -> L.index ts (p i)) (fun i -> index xs (p i))
+
+let apply_r_id_n (len : nat) (#ts : ty_list{L.length ts = len}) (xs :dlist ts)
+  : Lemma (apply_perm_r (Perm.id_n len) xs == xs) [SMTPat (apply_perm_r (Perm.id_n len) xs)]
+  = dlist_extensionality (apply_perm_r (Perm.id_n len) xs) xs
+
+let apply_r_comp (#len : nat) (f g : Perm.perm_f len) (#ts : ty_list {L.length ts == len}) (xs : dlist ts)
+  : Lemma (apply_perm_r (f `Perm.comp` g) xs === apply_perm_r f (apply_perm_r g xs))
+  = Perm.apply_r_comp f g ts;
+    dlist_extensionality (apply_perm_r (f `Perm.comp` g) xs) (apply_perm_r f (apply_perm_r g xs))
+
+let rec dlist_swap (i : nat) (#ts : ty_list{i <= L.length ts - 2}) (xs : dlist ts)
+  : Tot (dlist (Perm.list_swap i ts)) (decreases i)
+  = if i = 0
+    then let DCons tx x _ (DCons ty y _ tl) = xs in
+         DCons ty y _ (DCons tx x _ tl)
+    else let DCons tx x ts tl = xs in
+         DCons tx x _ (dlist_swap (i-1) tl)
+
+#push-options "--z3rlimit 20"
+let apply_perm_f_shift (#len : nat) (p : Perm.perm_f len)
+      (#hd_ty : Type) (#tl_ty : ty_list {L.length tl_ty = len})
+      (hd : hd_ty) (tl : dlist tl_ty)
+  : Lemma (apply_perm_r (Perm.perm_f_shift p) (DCons _ hd _ tl)
+       === DCons _ hd _ (apply_perm_r p tl))
+  = Perm.apply_perm_f_shift p hd_ty tl_ty;
+    dlist_extensionality
+      (apply_perm_r (Perm.perm_f_shift p) (DCons _ hd _ tl))
+      (DCons _ hd _ (apply_perm_r p tl))
+#pop-options
+
+#push-options "--z3rlimit 60"
+let rec apply_swap_as_rec (len : nat) (i : nat {i <= len-2})
+          (#ts : ty_list {L.length ts = len}) (xs : dlist ts)
+  : Lemma (ensures apply_perm_r (Perm.perm_f_swap #len i) xs === dlist_swap i xs)
+          (decreases len)
+  = Perm.apply_swap_as_rec len i ts;
+    if i = 0 then begin
+       let DCons _ x _ (DCons _ y _ tl) = xs in
+       dlist_extensionality
+         (apply_perm_r (Perm.perm_f_swap #len 0) (DCons _ x _ (DCons _ y _ tl)))
+         (DCons _ y _ (DCons _ x _ tl))
+    end else begin
+      let DCons _ hd _ tl = xs in
+      Perm.perm_f_swap_rec_rel (len-1) (i-1);
+      apply_perm_f_shift (Perm.perm_f_swap #(len-1) (i-1)) hd tl;
+      apply_swap_as_rec (len-1) (i-1) tl
+    end
+#pop-options
+
+
+unfold
+let apply_pequiv (#ts0 #ts1 : ty_list) (f : Perm.pequiv ts0 ts1) (xs : dlist ts0) : dlist ts1
+  = apply_perm_r f xs
+
+let apply_pequiv_sym_l (#ts0 #ts1 : ty_list) (f : Perm.pequiv ts0 ts1) (xs : dlist ts0)
+  : Lemma (apply_pequiv (Perm.pequiv_sym f) (apply_pequiv f xs) == xs)
+  =
+    apply_r_comp (Perm.inv_f f) f xs
+
+let apply_pequiv_sym_r (#ts0 #ts1 : ty_list) (f : Perm.pequiv ts0 ts1) (xs : dlist ts1)
+  : Lemma (apply_pequiv f (apply_pequiv (Perm.pequiv_sym f) xs) == xs)
+  =
+    Perm.pequiv_as_eq (Perm.pequiv_sym f);
+    apply_r_comp f (Perm.inv_f f) xs
+
+
+let apply_pequiv_sym_eq_iff (#ts0 #ts1 : ty_list) (f : Perm.pequiv ts0 ts1) (xs : dlist ts0) (ys : dlist ts1)
+  : Lemma (xs == apply_pequiv (Perm.pequiv_sym f) ys <==> ys == apply_pequiv f xs)
+  =
+    apply_pequiv_sym_l f xs;
+    apply_pequiv_sym_r f ys
